theories/program_logic/adequacy.v
@@ -1,0 +1,207 @@
+From iris_c.program_logic Require Export weakestpre.
+From iris.algebra Require Import gmap auth agree gset coPset.
+From iris.base_logic Require Import big_op soundness.
+From iris.base_logic.lib Require Import wsat.
+From iris.proofmode Require Import tactics.
+Set Default Proof Using "Type".
+Import uPred.
+
+(* Global functor setup *)
+Definition invΣ : gFunctors :=
+  #[GFunctor (authRF (gmapURF positive (agreeRF (laterCF idCF))));
+    GFunctor coPset_disjUR;
+    GFunctor (gset_disjUR positive)].
+
+Class invPreG (Σ : gFunctors) : Set := WsatPreG {
+  inv_inPreG :> inG Σ (authR (gmapUR positive (agreeR (laterC (iPreProp Σ)))));
+  enabled_inPreG :> inG Σ coPset_disjR;
+  disabled_inPreG :> inG Σ (gset_disjR positive);
+}.
+
+Instance subG_invΣ {Σ} : subG invΣ Σ → invPreG Σ.
+Proof. solve_inG. Qed.
+
+(* Allocation *)
+Lemma wsat_alloc `{invPreG Σ} : (|==> ∃ _ : invG Σ, wsat ∗ ownE ⊤)%I.
+Proof.
+  iIntros.
+  iMod (own_alloc (● (∅ : gmap _ _))) as (γI) "HI"; first done.
+  iMod (own_alloc (CoPset ⊤)) as (γE) "HE"; first done.
+  iMod (own_alloc (GSet ∅)) as (γD) "HD"; first done.
+  iModIntro; iExists (WsatG _ _ _ _ γI γE γD).
+  rewrite /wsat /ownE; iFrame.
+  iExists ∅. rewrite fmap_empty big_sepM_empty. by iFrame.
+Qed.
+
+(* Program logic adequacy *)
+Record adequate {Λ} (e1 : expr Λ) (l1: local_state Λ) (σ1 : state Λ) (φ : val Λ → Prop) := {
+  adequate_result t2 l2 σ2 v2 :
+   rtc step ([(e1, l1)], σ1) ((of_val v2, l2) :: t2, σ2) → φ v2;
+  adequate_safe t2 σ2 e2 l2 :
+   rtc step ([(e1, l1)], σ1) (t2, σ2) →
+   (e2, l2) ∈ t2 → (is_Some (to_val e2) ∨ reducible e2 l2 σ2)
+}.
+
+Theorem adequate_tp_safe {Λ} (e1 : expr Λ) l1 t2 σ1 σ2 φ :
+  adequate e1 l1 σ1 φ →
+  rtc step ([(e1, l1)], σ1) (t2, σ2) →
+  Forall (λ e, is_Some (to_val (e.1))) t2 ∨ ∃ t3 σ3, step (t2, σ2) (t3, σ3).
+Proof.
+  intros Had ?.
+  destruct (decide (Forall (λ e, is_Some (to_val (e.1))) t2)) as [|Ht2]; [by left|].
+  apply (not_Forall_Exists _), Exists_exists in Ht2; destruct Ht2 as ((e2&l2)&?&He2).
+  destruct (adequate_safe e1 l1 σ1 φ Had t2 σ2 e2 l2) as [?|(e3&l3&σ3&efs&?)];
+    rewrite ?eq_None_not_Some; auto.
+  { exfalso. eauto. }
+  destruct (elem_of_list_split t2 (e2, l2)) as (t2'&t2''&->); auto.
+  right; exists (t2' ++ (e3, l3) :: t2'' ++ (map (,init_local Λ) efs)), σ3; econstructor; eauto.
+Qed.
+
+Section adequacy.
+Context `{irisG Λ Σ}.
+Implicit Types e : expr Λ.
+Implicit Types P Q : iProp Σ.
+Implicit Types Φ : val Λ → iProp Σ.
+Implicit Types Φs : list (val Λ → iProp Σ).
+
+Notation world σ := (wsat ∗ ownE ⊤ ∗ state_interp σ)%I.
+
+Notation wptp t := ([∗ list] ef ∈ t, WP (ef.1) {{ _, True }})%I.
+
+Lemma wp_step e1 l1 σ1 e2 l2 σ2 efs Φ :
+  prim_step e1 l1 σ1 e2 l2 σ2 efs →
+  world σ1 ∗ WP e1 {{ Φ }} ==∗ ▷ |==> ◇ (world σ2 ∗ WP e2 {{ Φ }} ∗ wptp (map (,init_local Λ) efs)).
+Proof.
+  rewrite {1}wp_unfold /wp_pre. iIntros (Hstep) "[(Hw & HE & Hσ) [H|[_ H]]]".
+  { iDestruct "H" as (v) "[% _]". apply val_stuck in Hstep; simplify_eq. }
+  rewrite fupd_eq /fupd_def.
+  iMod ("H" $! l1 σ1 with "Hσ [Hw HE]") as ">(Hw & HE & _ & H)"; first by iFrame.
+  iModIntro; iNext.
+  iMod ("H" $! e2 l2 σ2 efs with "[%] [$Hw $HE]") as ">($ & $ & $ & $ & ?)"=>//.
+Admitted. (* apparent ... *)
+
+Lemma wptp_step e1 l1 t1 t2 σ1 σ2 Φ :
+  step ((e1, l1) :: t1,σ1) (t2, σ2) →
+  world σ1 ∗ WP e1 {{ Φ }} ∗ wptp t1
+  ==∗ ∃ e2 l2 t2', ⌜t2 = (e2, l2) :: t2'⌝ ∗ ▷ |==> ◇ (world σ2 ∗ WP e2 {{ Φ }} ∗ wptp t2').
+Proof.
+  iIntros (Hstep) "(HW & He & Ht)".
+  destruct Hstep as [e1' l1' σ1' e2' l2' σ2' efs [|? t1'] t2' ?? Hstep]; simplify_eq/=.
+  - iExists e2', l2', (t2' ++ map (,init_local Λ) efs); iSplitR; first eauto.
+    rewrite big_sepL_app. iFrame "Ht". iApply wp_step; try iFrame; eauto.
+  - iExists e1, l1, (t1' ++ (e2', l2') :: t2' ++ map (,init_local Λ) efs); iSplitR; first eauto.
+    rewrite !big_sepL_app !big_sepL_cons big_sepL_app.
+    iDestruct "Ht" as "($ & He' & $)"; iFrame "He". simpl.
+    iApply wp_step; try iFrame; eauto.
+Qed.
+
+Lemma wptp_steps n e1 l1 t1 t2 σ1 σ2 Φ :
+  nsteps step n ((e1, l1) :: t1, σ1) (t2, σ2) →
+  world σ1 ∗ WP e1 {{ Φ }} ∗ wptp t1 ⊢
+  Nat.iter (S n) (λ P, |==> ▷ P) (∃ e2 l2 t2',
+    ⌜t2 = (e2, l2) :: t2'⌝ ∗ world σ2 ∗ WP e2 {{ Φ }} ∗ wptp t2').
+Proof.
+  revert e1 l1 t1 t2 σ1 σ2; simpl; induction n as [|n IH]=> e1 l1 t1 t2 σ1 σ2 /=.
+  { inversion_clear 1; iIntros "?"; eauto 10. }
+  iIntros (Hsteps) "H". inversion_clear Hsteps as [|?? [t1' σ1']].
+  iMod (wptp_step with "H") as (e1' l1' t1'') "[% H]"; first eauto; simplify_eq.
+  iModIntro; iNext; iMod "H" as ">?". by iApply IH.
+Qed.
+
+Instance bupd_iter_mono n : Proper ((⊢) ==> (⊢)) (Nat.iter n (λ P, |==> ▷ P)%I).
+Proof. intros P Q HP. induction n; simpl; do 2?f_equiv; auto. Qed.
+
+Lemma bupd_iter_frame_l n R Q :
+  R ∗ Nat.iter n (λ P, |==> ▷ P) Q ⊢ Nat.iter n (λ P, |==> ▷ P) (R ∗ Q).
+Proof.
+  induction n as [|n IH]; simpl; [done|].
+  by rewrite bupd_frame_l {1}(later_intro R) -later_sep IH.
+Qed.
+
+Lemma wptp_result n e1 l1 l2 t1 v2 t2 σ1 σ2 φ :
+  nsteps step n ((e1, l1) :: t1, σ1) ((of_val v2, l2) :: t2, σ2) →
+  world σ1 ∗ WP e1 {{ v, ⌜φ v⌝ }} ∗ wptp t1 ⊢
+  Nat.iter (S (S n)) (λ P, |==> ▷ P) ⌜φ v2⌝.
+Proof.
+  intros. rewrite wptp_steps //.
+  rewrite (Nat_iter_S_r (S n)). apply bupd_iter_mono.
+  iDestruct 1 as (e2 l2' t2') "(% & (Hw & HE & _) & H & _)"; simplify_eq.
+  iDestruct (wp_value_inv with "H") as "H". rewrite fupd_eq /fupd_def.
+  iMod ("H" with "[Hw HE]") as ">(_ & _ & $)"; iFrame; auto.
+Qed.
+
+Lemma wp_safe e l σ Φ :
+  world σ ∗ WP e {{ Φ }} ==∗ ▷ ⌜is_Some (to_val e) ∨ reducible e l σ⌝.
+Proof.
+  rewrite wp_unfold /wp_pre. iIntros "[(Hw&HE&Hσ) [H|[_ H]]]".
+  { iDestruct "H" as (v) "[% _]"; eauto 10. }
+  rewrite fupd_eq. iMod ("H" with "* Hσ [-]") as ">(?&?&%&?)"; first by iFrame.
+  eauto 10.
+Qed.
+
+Lemma wptp_safe n e1 l1 e2 l2 t1 t2 σ1 σ2 Φ :
+  nsteps step n ((e1, l1) :: t1, σ1) (t2, σ2) → (e2, l2) ∈ t2 →
+  world σ1 ∗ WP e1 {{ Φ }} ∗ wptp t1 ⊢
+  Nat.iter (S (S n)) (λ P, |==> ▷ P) ⌜is_Some (to_val e2) ∨ reducible e2 l2 σ2⌝.
+Proof.
+  intros ? He2. rewrite wptp_steps //; rewrite (Nat_iter_S_r (S n)). apply bupd_iter_mono.
+  iDestruct 1 as (e2' l2' t2') "(% & Hw & H & Htp)"; simplify_eq.
+  apply elem_of_cons in He2 as [?|?]; first (inversion H0; subst; iApply wp_safe; by iFrame "Hw H").
+  iApply wp_safe. iFrame "Hw".
+  (* iApply (big_sepL_elem_of with "Htp"). *)
+Admitted.
+
+Lemma wptp_invariance n e1 l1 e2 t1 t2 σ1 σ2 φ Φ :
+  nsteps step n ((e1, l1) :: t1, σ1) (t2, σ2) →
+  (state_interp σ2 ={⊤,∅}=∗ ⌜φ⌝) ∗ world σ1 ∗ WP e1 {{ Φ }} ∗ wptp t1
+  ⊢ Nat.iter (S (S n)) (λ P, |==> ▷ P) ⌜φ⌝.
+Proof.
+  intros ?. rewrite wptp_steps //.
+  rewrite (Nat_iter_S_r (S n)) !bupd_iter_frame_l. apply bupd_iter_mono.
+  iIntros "[Hback H]".
+  iDestruct "H" as (e2' l2' t2') "(% & (Hw&HE&Hσ) & _)"; subst.
+  rewrite fupd_eq.
+  iMod ("Hback" with "Hσ [$Hw $HE]") as "> (_ & _ & $)"; auto.
+Qed.
+End adequacy.
+
+Theorem wp_adequacy Σ Λ `{invPreG Σ} e l σ φ :
+  (∀ `{Hinv : invG Σ},
+     True ={⊤}=∗ ∃ (stateI : state Λ → iProp Σ) (localI : local_state Λ → iProp Σ),
+       let _ : irisG Λ Σ := IrisG _ _ _ Hinv stateI localI in
+       stateI σ ∗ WP e {{ v, ⌜φ v⌝ }}) →
+  adequate e l σ φ.
+Proof.
+  intros Hwp; split.
+  - intros t2 l2 σ2 v2 [n ?]%rtc_nsteps.
+    eapply (soundness (M:=iResUR Σ) _ (S (S (S n)))); iIntros "".
+    rewrite Nat_iter_S. iMod wsat_alloc as (Hinv) "[Hw HE]".
+    rewrite fupd_eq in Hwp; iMod (Hwp with "[$Hw $HE]") as ">(Hw & HE & Hwp)".
+    iDestruct "Hwp" as (Istate Ilocal) "[HI Hwp]".
+    iModIntro. iNext. iApply (@wptp_result _ _ (IrisG _ _ _ Hinv Istate Ilocal)); eauto.
+    iFrame. by iApply big_sepL_nil.
+  - intros t2 l2 σ2 e2 [n ?]%rtc_nsteps ?.
+    eapply (soundness (M:=iResUR Σ) _ (S (S (S n)))); iIntros "".
+    rewrite Nat_iter_S. iMod wsat_alloc as (Hinv) "[Hw HE]".
+    rewrite fupd_eq in Hwp; iMod (Hwp with "[$Hw $HE]") as ">(Hw & HE & Hwp)".
+    iDestruct "Hwp" as (Istate Ilocal) "[HI Hwp]".
+    iModIntro. iNext. iApply (@wptp_safe _ _ (IrisG _ _ _ Hinv Istate Ilocal)); eauto.
+    iFrame. by iApply big_sepL_nil.
+Qed.
+
+Theorem wp_invariance Σ Λ `{invPreG Σ} e l σ1 t2 σ2 φ Φ :
+  (∀ `{Hinv : invG Σ},
+     True ={⊤}=∗ ∃ (stateI : state Λ → iProp Σ) (localI : local_state Λ → iProp Σ),
+       let _ : irisG Λ Σ := IrisG _ _ _ Hinv stateI localI in
+       stateI σ1 ∗ WP e {{ Φ }} ∗ (stateI σ2 ={⊤,∅}=∗ ⌜φ⌝)) →
+  rtc step ([(e, l)], σ1) (t2, σ2) →
+  φ.
+Proof.
+  intros Hwp [n ?]%rtc_nsteps.
+  eapply (soundness (M:=iResUR Σ) _ (S (S (S n)))); iIntros "".
+  rewrite Nat_iter_S. iMod wsat_alloc as (Hinv) "[Hw HE]".
+  rewrite {1}fupd_eq in Hwp; iMod (Hwp with "[$Hw $HE]") as ">(Hw & HE & Hwp)".
+  iDestruct "Hwp" as (Istate Ilocal) "(HIstate & Hwp & Hclose)".
+  iModIntro. iNext. iApply (@wptp_invariance _ _ (IrisG _ _ _ Hinv Istate Ilocal)); eauto.
+  iFrame "Hw HE Hwp HIstate Hclose". by iApply big_sepL_nil.
+Qed.
