theories/program_logic/hoare.v
@@ -1,0 +1,121 @@
+From iris_c.program_logic Require Export weakestpre.
+From iris.base_logic.lib Require Export viewshifts.
+From iris.proofmode Require Import tactics.
+Set Default Proof Using "Type".
+
+Definition ht `{irisG Λ Σ} (E : coPset) (P : iProp Σ)
+    (e : expr Λ) (Φ : val Λ → iProp Σ) : iProp Σ :=
+  (□ (P -∗ WP e @ E {{ Φ }}))%I.
+Instance: Params (@ht) 4.
+
+Notation "{{ P } } e @ E {{ Φ } }" := (ht E P%I e%E Φ%I)
+  (at level 20, P, e, Φ at level 200,
+   format "{{  P  } }  e  @  E  {{  Φ  } }") : C_scope.
+Notation "{{ P } } e {{ Φ } }" := (ht ⊤ P%I e%E Φ%I)
+  (at level 20, P, e, Φ at level 200,
+   format "{{  P  } }  e  {{  Φ  } }") : C_scope.
+
+Notation "{{ P } } e @ E {{ v , Q } }" := (ht E P%I e%E (λ v, Q)%I)
+  (at level 20, P, e, Q at level 200,
+   format "{{  P  } }  e  @  E  {{  v ,  Q  } }") : C_scope.
+Notation "{{ P } } e {{ v , Q } }" := (ht ⊤ P%I e%E (λ v, Q)%I)
+  (at level 20, P, e, Q at level 200,
+   format "{{  P  } }  e  {{  v ,  Q  } }") : C_scope.
+
+Section hoare.
+Context `{irisG Λ Σ}.
+Implicit Types P Q : iProp Σ.
+Implicit Types Φ Ψ : val Λ → iProp Σ.
+Implicit Types v : val Λ.
+Import uPred.
+
+Global Instance ht_ne E n :
+  Proper (dist n ==> eq==>pointwise_relation _ (dist n) ==> dist n) (ht E).
+Proof. solve_proper. Qed.
+Global Instance ht_proper E :
+  Proper ((≡) ==> eq ==> pointwise_relation _ (≡) ==> (≡)) (ht E).
+Proof. solve_proper. Qed.
+Lemma ht_mono E P P' Φ Φ' e :
+  (P ⊢ P') → (∀ v, Φ' v ⊢ Φ v) → {{ P' }} e @ E {{ Φ' }} ⊢ {{ P }} e @ E {{ Φ }}.
+Proof. by intros; apply always_mono, wand_mono, wp_mono. Qed.
+Global Instance ht_mono' E :
+  Proper (flip (⊢) ==> eq ==> pointwise_relation _ (⊢) ==> (⊢)) (ht E).
+Proof. solve_proper. Qed.
+
+Lemma ht_alt E P Φ e : (P ⊢ WP e @ E {{ Φ }}) → {{ P }} e @ E {{ Φ }}.
+Proof. iIntros (Hwp) "!# HP". by iApply Hwp. Qed.
+
+Lemma ht_val E v : {{ True }} of_val v @ E {{ v', ⌜v = v'⌝ }}.
+Proof. iIntros "!# _". by iApply wp_value'. Qed.
+
+Lemma ht_vs E P P' Φ Φ' e :
+  (P ={E}=> P') ∧ {{ P' }} e @ E {{ Φ' }} ∧ (∀ v, Φ' v ={E}=> Φ v)
+  ⊢ {{ P }} e @ E {{ Φ }}.
+Proof.
+  iIntros "(#Hvs & #Hwp & #HΦ) !# HP". iMod ("Hvs" with "HP") as "HP".
+  iApply wp_fupd. iApply (wp_wand with "[HP]"); [by iApply "Hwp"|].
+  iIntros (v) "Hv". by iApply "HΦ".
+Qed.
+
+Lemma ht_atomic E1 E2 P P' Φ Φ' e :
+  atomic e →
+  (P ={E1,E2}=> P') ∧ {{ P' }} e @ E2 {{ Φ' }} ∧ (∀ v, Φ' v ={E2,E1}=> Φ v)
+  ⊢ {{ P }} e @ E1 {{ Φ }}.
+Proof.
+  iIntros (?) "(#Hvs & #Hwp & #HΦ) !# HP". iApply (wp_atomic _ E2); auto.
+  iMod ("Hvs" with "HP") as "HP". iModIntro.
+  iApply (wp_wand with "[HP]"); [by iApply "Hwp"|].
+  iIntros (v) "Hv". by iApply "HΦ".
+Qed.
+
+Lemma ht_mask_weaken E1 E2 P Φ e :
+  E1 ⊆ E2 → {{ P }} e @ E1 {{ Φ }} ⊢ {{ P }} e @ E2 {{ Φ }}.
+Proof.
+  iIntros (?) "#Hwp !# HP". iApply (wp_mask_mono E1 E2); try done.
+  by iApply "Hwp".
+Qed.
+
+Lemma ht_frame_l E P Φ R e :
+  {{ P }} e @ E {{ Φ }} ⊢ {{ R ∗ P }} e @ E {{ v, R ∗ Φ v }}.
+Proof. iIntros "#Hwp !# [$ HP]". by iApply "Hwp". Qed.
+
+Lemma ht_frame_r E P Φ R e :
+  {{ P }} e @ E {{ Φ }} ⊢ {{ P ∗ R }} e @ E {{ v, Φ v ∗ R }}.
+Proof. iIntros "#Hwp !# [HP $]". by iApply "Hwp". Qed.
+
+Lemma ht_frame_step_l E1 E2 P R1 R2 e Φ :
+  to_val e = None → E2 ⊆ E1 →
+  (R1 ={E1,E2}=> ▷ |={E2,E1}=> R2) ∧ {{ P }} e @ E2 {{ Φ }}
+  ⊢ {{ R1 ∗ P }} e @ E1 {{ λ v, R2 ∗ Φ v }}.
+Proof.
+  iIntros (??) "[#Hvs #Hwp] !# [HR HP]".
+  iApply (wp_frame_step_l E1 E2); try done.
+  iSplitL "HR"; [by iApply "Hvs"|by iApply "Hwp"].
+Qed.
+
+Lemma ht_frame_step_r E1 E2 P R1 R2 e Φ :
+  to_val e = None → E2 ⊆ E1 →
+  (R1 ={E1,E2}=> ▷ |={E2,E1}=> R2) ∧ {{ P }} e @ E2 {{ Φ }}
+  ⊢ {{ P ∗ R1 }} e @ E1 {{ λ v, Φ v ∗ R2 }}.
+Proof.
+  iIntros (??) "[#Hvs #Hwp] !# [HP HR]".
+  iApply (wp_frame_step_r E1 E2); try done.
+  iSplitR "HR"; [by iApply "Hwp"|by iApply "Hvs"].
+Qed.
+
+Lemma ht_frame_step_l' E P R e Φ :
+  to_val e = None →
+  {{ P }} e @ E {{ Φ }} ⊢ {{ ▷ R ∗ P }} e @ E {{ v, R ∗ Φ v }}.
+Proof.
+  iIntros (?) "#Hwp !# [HR HP]".
+  iApply wp_frame_step_l'; try done. iFrame "HR". by iApply "Hwp".
+Qed.
+
+Lemma ht_frame_step_r' E P Φ R e :
+  to_val e = None →
+  {{ P }} e @ E {{ Φ }} ⊢ {{ P ∗ ▷ R }} e @ E {{ v, Φ v ∗ R }}.
+Proof.
+  iIntros (?) "#Hwp !# [HP HR]".
+  iApply wp_frame_step_r'; try done. iFrame "HR". by iApply "Hwp".
+Qed.
+End hoare.
