theories/program_logic/language.v
@@ -1,0 +1,60 @@
+From iris.algebra Require Export ofe.
+Set Default Proof Using "Type".
+
+Structure language := Language {
+  expr : Type;
+  val : Type;
+  local_state : Type;
+  state : Type;
+  of_val : val → expr;
+  to_val : expr → option val;
+  init_local: local_state;
+  prim_step : expr → local_state → state → expr → local_state → state → list expr → Prop;
+  to_of_val v : to_val (of_val v) = Some v;
+  of_to_val e v : to_val e = Some v → of_val v = e;
+  val_stuck e l σ e' l' σ' efs : prim_step e l σ e' l' σ' efs → to_val e = None
+}.
+Delimit Scope expr_scope with E.
+Delimit Scope val_scope with V.
+Bind Scope expr_scope with expr.
+Bind Scope val_scope with val.
+Arguments of_val {_} _.
+Arguments to_val {_} _.
+Arguments prim_step {_} _ _ _ _ _ _ _.
+Arguments to_of_val {_} _.
+Arguments of_to_val {_} _ _ _.
+Arguments val_stuck {_} _ _ _ _ _ _ _ _.
+
+Canonical Structure stateC Λ := leibnizC (state Λ).
+Canonical Structure local_stateC Λ := leibnizC (local_state Λ).
+Canonical Structure valC Λ := leibnizC (val Λ).
+Canonical Structure exprC Λ := leibnizC (expr Λ).
+
+Definition cfg (Λ : language) := (list (expr Λ * local_state Λ) * state Λ)%type.
+
+Section language.
+  Context {Λ : language}.
+  Implicit Types v : val Λ.
+
+  Definition reducible (e : expr Λ) (l: local_state Λ) (σ : state Λ) :=
+    ∃ e' l' σ' efs, prim_step e l σ e' l' σ' efs.
+  Definition irreducible (e : expr Λ) (l: local_state Λ) (σ : state Λ) :=
+    ∀ e' l' σ' efs, ¬prim_step e l σ e' l' σ' efs.
+  Definition atomic (e : expr Λ) : Prop :=
+    ∀ l σ e' l' σ' efs, prim_step e l σ e' l' σ' efs → irreducible e' l' σ'.
+  Inductive step (ρ1 ρ2 : cfg Λ) : Prop :=
+    | step_atomic e1 l1 σ1 e2 l2 σ2 efs t1 t2 :
+       ρ1 = (t1 ++ (e1, l1) :: t2, σ1) →
+       ρ2 = (t1 ++ (e2, l2) :: t2 ++ map (,init_local Λ) efs, σ2) →
+       prim_step e1 l1 σ1 e2 l2 σ2 efs →
+       step ρ1 ρ2.
+
+  Lemma of_to_val_flip v e : of_val v = e → to_val e = Some v.
+  Proof. intros <-. by rewrite to_of_val. Qed.
+  Lemma reducible_not_val e l σ : reducible e l σ → to_val e = None.
+  Proof. intros (?&?&?&?&?); eauto using val_stuck. Qed.
+  Lemma val_irreducible e l σ : is_Some (to_val e) → irreducible e l σ.
+  Proof. intros [??] ???? ?%val_stuck. by destruct (to_val e). Qed.
+  Global Instance of_val_inj : Inj (=) (=) (@of_val Λ).
+  Proof. by intros v v' Hv; apply (inj Some); rewrite -!to_of_val Hv. Qed.
+End language.
