theories/program_logic/weakestpre.v
@@ -1,0 +1,287 @@
+From iris.base_logic.lib Require Export fancy_updates.
+From iris_c.program_logic Require Export language.
+From iris.base_logic Require Import big_op.
+From iris.proofmode Require Import tactics classes.
+Set Default Proof Using "Type".
+Import uPred.
+
+Class irisG' (Λlocal Λstate : Type) (Σ : gFunctors) := IrisG {
+  iris_invG :> invG Σ;
+  state_interp : Λstate → iProp Σ;
+  local_interp : Λlocal → iProp Σ;
+}.
+Notation irisG Λ Σ := (irisG' (local_state Λ) (state Λ) Σ).
+
+Definition wp_pre `{irisG Λ Σ}
+    (wp : coPset -c> expr Λ -c> (val Λ -c> iProp Σ) -c> iProp Σ) :
+    coPset -c> expr Λ -c> (val Λ -c> iProp Σ) -c> iProp Σ := λ E e1 Φ, (
+  (* value case *)
+  (∃ v, ⌜to_val e1 = Some v⌝ ∧ |={E}=> Φ v) ∨
+  (* step case *)
+  (⌜to_val e1 = None⌝ ∧ ∀ l1 σ1,
+     state_interp σ1 ∗ local_interp l1 ={E,∅}=∗ ⌜reducible e1 l1 σ1⌝ ∗
+     ▷ ∀ e2 l2 σ2 efs, ⌜prim_step e1 l1 σ1 e2 l2 σ2 efs⌝ ={∅,E}=∗
+       state_interp σ2 ∗ local_interp l2 ∗ wp E e2 Φ ∗
+       [∗ list] ef ∈ efs, local_interp (init_local Λ) -∗ wp ⊤ ef (λ _, True)))%I.
+
+Local Instance wp_pre_contractive `{irisG Λ Σ} : Contractive wp_pre.
+Proof.
+  rewrite /wp_pre=> n wp wp' Hwp E e1 Φ.
+  repeat (f_contractive || f_equiv); apply Hwp.
+Qed.
+
+Definition wp_def `{irisG Λ Σ} :
+  coPset → expr Λ → (val Λ → iProp Σ) → iProp Σ := fixpoint wp_pre.
+Definition wp_aux : { x | x = @wp_def }. by eexists. Qed.
+Definition wp := proj1_sig wp_aux.
+Definition wp_eq : @wp = @wp_def := proj2_sig wp_aux.
+
+Arguments wp {_ _ _} _ _%E _.
+Instance: Params (@wp) 5.
+
+Notation "'WP' e @ E {{ Φ } }" := (wp E e%E Φ)
+  (at level 20, e, Φ at level 200,
+   format "'WP'  e  @  E  {{  Φ  } }") : uPred_scope.
+Notation "'WP' e {{ Φ } }" := (wp ⊤ e%E Φ)
+  (at level 20, e, Φ at level 200,
+   format "'WP'  e  {{  Φ  } }") : uPred_scope.
+
+Notation "'WP' e @ E {{ v , Q } }" := (wp E e%E (λ v, Q))
+  (at level 20, e, Q at level 200,
+   format "'WP'  e  @  E  {{  v ,  Q  } }") : uPred_scope.
+Notation "'WP' e {{ v , Q } }" := (wp ⊤ e%E (λ v, Q))
+  (at level 20, e, Q at level 200,
+   format "'WP'  e  {{  v ,  Q  } }") : uPred_scope.
+
+(* Texan triples *)
+Notation "'{{{' P } } } e {{{ x .. y , 'RET' pat ; Q } } }" :=
+  (□ ∀ Φ,
+      P -∗ ▷ (∀ x, .. (∀ y, Q -∗ Φ pat%V) .. ) -∗ WP e {{ Φ }})%I
+    (at level 20, x closed binder, y closed binder,
+     format "{{{  P  } } }  e  {{{  x .. y ,   RET  pat ;  Q } } }") : uPred_scope.
+Notation "'{{{' P } } } e @ E {{{ x .. y , 'RET' pat ; Q } } }" :=
+  (□ ∀ Φ,
+      P -∗ ▷ (∀ x, .. (∀ y, Q -∗ Φ pat%V) .. ) -∗ WP e @ E {{ Φ }})%I
+    (at level 20, x closed binder, y closed binder,
+     format "{{{  P  } } }  e  @  E  {{{  x .. y ,  RET  pat ;  Q } } }") : uPred_scope.
+Notation "'{{{' P } } } e {{{ 'RET' pat ; Q } } }" :=
+  (□ ∀ Φ, P -∗ ▷ (Q -∗ Φ pat%V) -∗ WP e {{ Φ }})%I
+    (at level 20,
+     format "{{{  P  } } }  e  {{{  RET  pat ;  Q } } }") : uPred_scope.
+Notation "'{{{' P } } } e @ E {{{ 'RET' pat ; Q } } }" :=
+  (□ ∀ Φ, P -∗ ▷ (Q -∗ Φ pat%V) -∗ WP e @ E {{ Φ }})%I
+    (at level 20,
+     format "{{{  P  } } }  e  @  E  {{{  RET  pat ;  Q } } }") : uPred_scope.
+
+Notation "'{{{' P } } } e {{{ x .. y , 'RET' pat ; Q } } }" :=
+  (∀ Φ : _ → uPred _,
+      P -∗ ▷ (∀ x, .. (∀ y, Q -∗ Φ pat%V) .. ) -∗ WP e {{ Φ }})
+    (at level 20, x closed binder, y closed binder,
+     format "{{{  P  } } }  e  {{{  x .. y ,  RET  pat ;  Q } } }") : C_scope.
+Notation "'{{{' P } } } e @ E {{{ x .. y , 'RET' pat ; Q } } }" :=
+  (∀ Φ : _ → uPred _,
+      P -∗ ▷ (∀ x, .. (∀ y, Q -∗ Φ pat%V) .. ) -∗ WP e @ E {{ Φ }})
+    (at level 20, x closed binder, y closed binder,
+     format "{{{  P  } } }  e  @  E  {{{  x .. y ,  RET  pat ;  Q } } }") : C_scope.
+Notation "'{{{' P } } } e {{{ 'RET' pat ; Q } } }" :=
+  (∀ Φ : _ → uPred _, P -∗ ▷ (Q -∗ Φ pat%V) -∗ WP e {{ Φ }})
+    (at level 20,
+     format "{{{  P  } } }  e  {{{  RET  pat ;  Q } } }") : C_scope.
+Notation "'{{{' P } } } e @ E {{{ 'RET' pat ; Q } } }" :=
+  (∀ Φ : _ → uPred _, P -∗ ▷ (Q -∗ Φ pat%V) -∗ WP e @ E {{ Φ }})
+    (at level 20,
+     format "{{{  P  } } }  e  @  E  {{{  RET  pat ;  Q } } }") : C_scope.
+
+Section wp.
+Context `{irisG Λ Σ}.
+Implicit Types P : iProp Σ.
+Implicit Types Φ : val Λ → iProp Σ.
+Implicit Types v : val Λ.
+Implicit Types e : expr Λ.
+
+(* Weakest pre *)
+Lemma wp_unfold E e Φ : WP e @ E {{ Φ }} ⊣⊢ wp_pre wp E e Φ.
+Proof. rewrite wp_eq. apply (fixpoint_unfold wp_pre). Qed.
+
+Global Instance wp_ne E e n :
+  Proper (pointwise_relation _ (dist n) ==> dist n) (@wp Λ Σ _ E e).
+Proof.
+  revert e. induction (lt_wf n) as [n _ IH]=> e Φ Ψ HΦ.
+  rewrite !wp_unfold /wp_pre.
+  (* FIXME: figure out a way to properly automate this proof *)
+  (* FIXME: reflexivity, as being called many times by f_equiv and f_contractive
+  is very slow here *)
+  do 23 (f_contractive || f_equiv). apply IH; first lia.
+  intros v. eapply dist_le; eauto with omega.
+Qed.
+Global Instance wp_proper E e :
+  Proper (pointwise_relation _ (≡) ==> (≡)) (@wp Λ Σ _ E e).
+Proof.
+  by intros Φ Φ' ?; apply equiv_dist=>n; apply wp_ne=>v; apply equiv_dist.
+Qed.
+
+Lemma wp_value' E Φ v : Φ v ⊢ WP of_val v @ E {{ Φ }}.
+Proof.
+  iIntros "HΦ". rewrite wp_unfold /wp_pre.
+  iLeft; iExists v; rewrite to_of_val; auto.
+Qed.
+Lemma wp_value_inv E Φ v : WP of_val v @ E {{ Φ }} ={E}=∗ Φ v.
+Proof.
+  rewrite wp_unfold /wp_pre to_of_val. iIntros "[H|[% _]]"; [|done].
+  by iDestruct "H" as (v') "[% ?]"; simplify_eq.
+Qed.
+
+Lemma wp_strong_mono E1 E2 e Φ Ψ :
+  E1 ⊆ E2 → (∀ v, Φ v ={E2}=∗ Ψ v) ∗ WP e @ E1 {{ Φ }} ⊢ WP e @ E2 {{ Ψ }}.
+Proof.
+  iIntros (?) "[HΦ H]". iLöb as "IH" forall (e). rewrite !wp_unfold /wp_pre.
+  iDestruct "H" as "[Hv|[% H]]"; [iLeft|iRight].
+  { iDestruct "Hv" as (v) "[% Hv]". iExists v; iSplit; first done.
+    iApply ("HΦ" with ">[-]"). by iApply (fupd_mask_mono E1 _). }
+  iSplit; [done|]; iIntros (l1 σ1) "Hσ".
+  iMod (fupd_intro_mask' E2 E1) as "Hclose"; first done.
+  iMod ("H" $! l1 σ1 with "Hσ") as "[$ H]".
+  iModIntro. iNext. iIntros (e2 l2 σ2 efs Hstep).
+  iMod ("H" $! _ _ _ efs with "[#]") as "($ & $ & H & $)"; auto.
+  iMod "Hclose" as "_". by iApply ("IH" with "HΦ").
+Qed.
+
+Lemma fupd_wp E e Φ : (|={E}=> WP e @ E {{ Φ }}) ⊢ WP e @ E {{ Φ }}.
+Proof.
+  rewrite wp_unfold /wp_pre. iIntros "H". destruct (to_val e) as [v|] eqn:?.
+  { iLeft. iExists v; iSplit; first done.
+    by iMod "H" as "[H|[% ?]]"; [iDestruct "H" as (v') "[% ?]"|]; simplify_eq. }
+  iRight; iSplit; [done|]; iIntros (l1 σ1) "Hσ1".
+  iMod "H" as "[H|[% H]]"; last by iApply "H".
+  iDestruct "H" as (v') "[% ?]"; simplify_eq.
+Qed.
+Lemma wp_fupd E e Φ : WP e @ E {{ v, |={E}=> Φ v }} ⊢ WP e @ E {{ Φ }}.
+Proof. iIntros "H". iApply (wp_strong_mono E); try iFrame; auto. Qed.
+
+Lemma wp_atomic E1 E2 e Φ :
+  atomic e →
+  (|={E1,E2}=> WP e @ E2 {{ v, |={E2,E1}=> Φ v }}) ⊢ WP e @ E1 {{ Φ }}.
+Proof.
+  iIntros (Hatomic) "H". destruct (to_val e) as [v|] eqn:He.
+  { apply of_to_val in He as <-. iApply wp_fupd. iApply wp_value'.
+    iMod "H". by iMod (wp_value_inv with "H"). }
+  setoid_rewrite wp_unfold; rewrite /wp_pre. iRight; iSplit; auto.
+  iIntros (l1 σ1) "Hσ". iMod "H" as "[H|[_ H]]".
+  { iDestruct "H" as (v') "[% ?]"; simplify_eq. }
+  iMod ("H" $! _ _ with "Hσ") as "[$ H]".
+  iModIntro. iNext. iIntros (e2 l2 σ2 efs Hstep).
+  iMod ("H" with "* []") as "(Hphy & Hl & H & $)"; first done.
+  rewrite wp_unfold /wp_pre. iDestruct "H" as "[H|H]".
+  - iDestruct "H" as (v) "[% >>?]". iModIntro. iFrame.
+    rewrite -(of_to_val e2 v) //. by iApply wp_value'.
+  - iDestruct "H" as "[_ H]".
+    iMod ("H" with "* [Hphy Hl]") as "[H _]"; first iFrame.
+    iDestruct "H" as %(? & ? & ? & ? & ?). exfalso.
+    by eapply (Hatomic _ _ _ _ _ _ Hstep).
+Qed.
+
+Lemma wp_fupd_step E1 E2 e P Φ :
+  to_val e = None → E2 ⊆ E1 →
+  (|={E1,E2}▷=> P) -∗ WP e @ E2 {{ v, P ={E1}=∗ Φ v }} -∗ WP e @ E1 {{ Φ }}.
+Proof.
+  rewrite !wp_unfold /wp_pre. iIntros (??) "HR [Hv|[_ H]]".
+  { iDestruct "Hv" as (v) "[% Hv]"; simplify_eq. }
+  iRight; iSplit; [done|]. iIntros (l1 σ1) "[Hσ Hl]".
+  iMod "HR". iMod ("H" $! _ _ with "[Hσ Hl]") as "[$ H]"; first iFrame.
+  iModIntro; iNext; iIntros (e2 l2 σ2 efs Hstep).
+  iMod ("H" $! e2 l2 σ2 efs with "[%]") as "($ & $ & H & $)"; auto=>//.
+  iMod "HR". iModIntro. iApply (wp_strong_mono E2); first done.
+  iSplitR "H"; last iExact "H". iIntros (v) "H". by iApply "H".
+Qed.
+
+(** * Derived rules *)
+Lemma wp_mono E e Φ Ψ : (∀ v, Φ v ⊢ Ψ v) → WP e @ E {{ Φ }} ⊢ WP e @ E {{ Ψ }}.
+Proof.
+  iIntros (HΦ) "H"; iApply (wp_strong_mono E E); auto.
+  iFrame. iIntros (v) "?". by iApply HΦ.
+Qed.
+Lemma wp_mask_mono E1 E2 e Φ : E1 ⊆ E2 → WP e @ E1 {{ Φ }} ⊢ WP e @ E2 {{ Φ }}.
+Proof. iIntros (?) "H"; iApply (wp_strong_mono E1 E2); auto. iFrame; eauto. Qed.
+Global Instance wp_mono' E e :
+  Proper (pointwise_relation _ (⊢) ==> (⊢)) (@wp Λ Σ _ E e).
+Proof. by intros Φ Φ' ?; apply wp_mono. Qed.
+
+Lemma wp_value E Φ e v : to_val e = Some v → Φ v ⊢ WP e @ E {{ Φ }}.
+Proof. intros; rewrite -(of_to_val e v) //; by apply wp_value'. Qed.
+Lemma wp_value_fupd' E Φ v : (|={E}=> Φ v) ⊢ WP of_val v @ E {{ Φ }}.
+Proof. intros. by rewrite -wp_fupd -wp_value'. Qed.
+Lemma wp_value_fupd E Φ e v :
+  to_val e = Some v → (|={E}=> Φ v) ⊢ WP e @ E {{ Φ }}.
+Proof. intros. rewrite -wp_fupd -wp_value //. Qed.
+
+Lemma wp_frame_l E e Φ R : R ∗ WP e @ E {{ Φ }} ⊢ WP e @ E {{ v, R ∗ Φ v }}.
+Proof. iIntros "[??]". iApply (wp_strong_mono E E _ Φ); try iFrame; eauto. Qed.
+Lemma wp_frame_r E e Φ R : WP e @ E {{ Φ }} ∗ R ⊢ WP e @ E {{ v, Φ v ∗ R }}.
+Proof. iIntros "[??]". iApply (wp_strong_mono E E _ Φ); try iFrame; eauto. Qed.
+
+Lemma wp_frame_step_l E1 E2 e Φ R :
+  to_val e = None → E2 ⊆ E1 →
+  (|={E1,E2}▷=> R) ∗ WP e @ E2 {{ Φ }} ⊢ WP e @ E1 {{ v, R ∗ Φ v }}.
+Proof.
+  iIntros (??) "[Hu Hwp]". iApply (wp_fupd_step with "Hu"); try done.
+  iApply (wp_mono with "Hwp"). by iIntros (?) "$$".
+Qed.
+Lemma wp_frame_step_r E1 E2 e Φ R :
+  to_val e = None → E2 ⊆ E1 →
+  WP e @ E2 {{ Φ }} ∗ (|={E1,E2}▷=> R) ⊢ WP e @ E1 {{ v, Φ v ∗ R }}.
+Proof.
+  rewrite [(WP _ @ _ {{ _ }} ∗ _)%I]comm; setoid_rewrite (comm _ _ R).
+  apply wp_frame_step_l.
+Qed.
+Lemma wp_frame_step_l' E e Φ R :
+  to_val e = None → ▷ R ∗ WP e @ E {{ Φ }} ⊢ WP e @ E {{ v, R ∗ Φ v }}.
+Proof. iIntros (?) "[??]". iApply (wp_frame_step_l E E); try iFrame; eauto. Qed.
+Lemma wp_frame_step_r' E e Φ R :
+  to_val e = None → WP e @ E {{ Φ }} ∗ ▷ R ⊢ WP e @ E {{ v, Φ v ∗ R }}.
+Proof. iIntros (?) "[??]". iApply (wp_frame_step_r E E); try iFrame; eauto. Qed.
+
+Lemma wp_wand E e Φ Ψ :
+  WP e @ E {{ Φ }} -∗ (∀ v, Φ v -∗ Ψ v) -∗ WP e @ E {{ Ψ }}.
+Proof.
+  iIntros "Hwp H". iApply (wp_strong_mono E); auto.
+  iFrame "Hwp". iIntros (?) "?". by iApply "H".
+Qed.
+Lemma wp_wand_l E e Φ Ψ :
+  (∀ v, Φ v -∗ Ψ v) ∗ WP e @ E {{ Φ }} ⊢ WP e @ E {{ Ψ }}.
+Proof. iIntros "[H Hwp]". iApply (wp_wand with "Hwp H"). Qed.
+Lemma wp_wand_r E e Φ Ψ :
+  WP e @ E {{ Φ }} ∗ (∀ v, Φ v -∗ Ψ v) ⊢ WP e @ E {{ Ψ }}.
+Proof. iIntros "[Hwp H]". iApply (wp_wand with "Hwp H"). Qed.
+End wp.
+
+(** Proofmode class instances *)
+Section proofmode_classes.
+  Context `{irisG Λ Σ}.
+  Implicit Types P Q : iProp Σ.
+  Implicit Types Φ : val Λ → iProp Σ.
+
+  Global Instance frame_wp E e R Φ Ψ :
+    (∀ v, Frame R (Φ v) (Ψ v)) → Frame R (WP e @ E {{ Φ }}) (WP e @ E {{ Ψ }}).
+  Proof. rewrite /Frame=> HR. rewrite wp_frame_l. apply wp_mono, HR. Qed.
+
+  Global Instance is_except_0_wp E e Φ : IsExcept0 (WP e @ E {{ Φ }}).
+  Proof. by rewrite /IsExcept0 -{2}fupd_wp -except_0_fupd -fupd_intro. Qed.
+
+  Global Instance elim_modal_bupd_wp E e P Φ :
+    ElimModal (|==> P) P (WP e @ E {{ Φ }}) (WP e @ E {{ Φ }}).
+  Proof. by rewrite /ElimModal (bupd_fupd E) fupd_frame_r wand_elim_r fupd_wp. Qed.
+
+  Global Instance elim_modal_fupd_wp E e P Φ :
+    ElimModal (|={E}=> P) P (WP e @ E {{ Φ }}) (WP e @ E {{ Φ }}).
+  Proof. by rewrite /ElimModal fupd_frame_r wand_elim_r fupd_wp. Qed.
+
+  (* lower precedence, if possible, it should always pick elim_upd_fupd_wp *)
+  Global Instance elim_modal_fupd_wp_atomic E1 E2 e P Φ :
+    atomic e →
+    ElimModal (|={E1,E2}=> P) P
+            (WP e @ E1 {{ Φ }}) (WP e @ E2 {{ v, |={E2,E1}=> Φ v }})%I | 100.
+  Proof. intros. by rewrite /ElimModal fupd_frame_r wand_elim_r wp_atomic. Qed.
+
+End proofmode_classes.
+
+Hint Extern 0 (atomic _) => assumption : typeclass_instances.
